- $S_n = -S_{n-1} + 10$ with initial condition $S_0 = 4$
  
  *Ignore the initial condition!*
  We're going to instead look it symbolically, as that's what allows us to analyze our recurrence relations for an emerging pattern. 
  
  $S_0=x$
  $S_1=-(S_0)+10$ or $S_1=-(x)+10$
  $S_2=-(S_1)+10$ or $S_2=-(-(x)+10)+10$
  $S_3=-(S_2)+10$ or $S_3=-(-(-(x)+10)+10)+10$
  
  By $S_3$, we see a pattern. There's 3 negatives ones multiplied to the first x, 2 negatives ones multiplied to the first ten, 1 negative one multiplied to the second ten, and 0 negative ones multiplied to the third ten.
  
  Therefore, we can generalize this pattern:
  $S_n=(-1)^{n}x+(-1)^{n-1}10+(-1)^{n-2}10+...+(-1)^{0}10$
  
  Don't forget to replace our symbolic $x$ with $S_0$:
  $$S_n=(-1)^{n}S_0+(-1)^{n-1}10+(-1)^{n-2}10+...+(-1)^{0}10$$
-