### Differential Equation
Equation which relates an unknown function x(t) and its derivatives.
	- ### Example
	  $$\frac{dx}{dt}+t^3x(t)=1$$
	  **Standard Form**: $$\frac{dx}{dt}=1-t^3x(t)$$
- ### Separable Differential Equations
  $$\frac{dy}{dx}=f(x,y(x))=h(x)*g(y)$$
	- ###  Types
	  $$\frac{dy}{dx}=e^{x+y}$$
	  Separable (is a product)
	  $$\frac{dy}{dx}=x-2y$$
	  Not separable (not a product)
	- ### Example Problem
	  $$x\frac{dy}{dx}-1=y^2$$
	  $$\text{or}$$
	  $$\frac{dy}{dx}=\frac{1}{x}(1+y^2)$$
	  $$\text{or}$$
	  $$\int{\frac{1}{1+y^2}}dy=\int{\frac{1}{x}}dx$$
	  $$\text{or}$$
	  $$y(x)=\tan{(\ln{|x|}+C)}$$
	  And if we consider an initial condition y(1) = 0,
	  $$0=\tan{C}$$
	  $$\text{or}$$
	  $$C=0$$
	  $$\text{so}$$
	  $$y(x)=\tan(\ln|x|)$$
- ## Principle Problem
  Let P(t) = population at time t=0.
  $\frac{dp}{dt}$ = rate of change for P(t)
  
  General population model:
  $\beta(p)$ = birth rate per individual per unit of time
  $\delta(p)$ = death rate per individual per unit of time
  $\frac{dp}{dt}=(\beta(p)-\delta(p))p$
  
  ** Notable Scenario: **
  * \delta(p)=0 and \beta(p) > 0: Exponential growth, strictly increasing
  Solving: 
  $$\frac{dp}{dt}=kP$$
  $$\text{or}$$
  $$\int \frac{1}{p} dp = \int kdt$$
  $$\text{or}$$
  $$\ln|p|=kt+C$$
  $$\text{or}$$
  $$p(t)=\pm e^c e^{kt} \text{ or } p(t) = Ce^{kt}$$
  $$\text{so (by solving for C in the above equation with the initial condition p(t0)=p0)}$$
  $$p(t)=P_0e^{k(t-t_0)}$$
  
  Allowing:
  $\beta=\beta_0+\beta_1p$
  $\delta=\delta_0+\delta_1p$
  $$\frac{dp}{dt}=(\beta_0+\beta_1p-(\delta_0+\delta_1p))p$$
  $$=-(\beta_1-\delta_1)(-\frac{\beta_0-\delta_0}{\beta_1-\delta_1}-p)p$$
	- ### Logistic Model Growth
	  $$\frac{dP}{dt}=k(M-P)P, k > 0, M > 0$$
	  $$P(t_0)=P_0$$
	  $$\text{(M = Carrying Capacity)}$$
	  
	  Seperating:
	  $$\frac{dP}{(M-P)P}=(k)dt$$
	  $$\text{or}$$
	  $$\int \frac{dP}{(M-P)P}=kt + C$$
	  $$\text{Using integration by fractional seperation}$$
	  $$\frac{1}{M}\int (\frac{1}{P} + \frac{1}{(M-P)})dP=kt+C$$
	  $$\text{or}$$
	  $$\frac{1}{M}(ln|P|-ln|M-P|)=kt+C$$
	  $$\text{or}$$
	  $$\frac{1}{M}(ln|P}{M-P}|)=kt+C$$
	  Next, we must find C using our initial condition specified above ($P(t_0)=P_0$)